projection simps

src/computational_monads/simulation_semantics/constructions/stateless_oracle.lean
@@ -1,59 +1,11 @@
 import computational_monads.constructions.uniform_select
 import computational_monads.simulation_semantics.simulate
+import computational_monads.simulation_semantics.constructions.tracking_oracle
 
 open oracle_comp oracle_spec
 
 variables {A B : Type} {spec spec' spec'' : oracle_spec}
   (oa : oracle_comp spec A)
-
--- TODO: use namespaces to simplify the lemma names
-
-section tracking_oracle
-
-/-- Oracle where the query result is indepenent of the current oracle state,
-  although the new state may depend upon the previous state.
-  For example a logging oracle that just tracks the input and output of queries. -/
-def tracking_oracle {S : Type} (default_state : S)
-  (o : Π (i : spec.ι), spec.domain i → oracle_comp spec' (spec.range i))
-  (update_state : Π (s : S) (i : spec.ι), spec.domain i → spec.range i → S) :
-  simulation_oracle spec spec' :=
-{ S := S,
-  default_state := default_state,
-  o := λ i ⟨t, s⟩, do { u ← o i t, pure (u, update_state s i t u) } }
-
-notation `⟪` o `|` update_state `,` default_state `⟫` :=
-  tracking_oracle default_state o update_state
-
-variables {S : Type} (default_state : S)
-  (o : Π (i : spec.ι), spec.domain i → oracle_comp spec' (spec.range i))
-  (update_state : Π (s : S) (i : spec.ι), spec.domain i → spec.range i → S)
-
-@[simp]
-lemma default_state_tracking_oracle :
-  (⟪o | update_state, default_state⟫).default_state = default_state := rfl
-
-@[simp]
-lemma tracking_oracle_apply (i : spec.ι) (t : spec.domain i) (s : S) :
-  (⟪o | update_state, default_state⟫).o i (t, s) =
-    do { u ← o i t, pure (u, update_state s i t u) } := rfl
-
--- TODO: should be able to find some generalization for lemmas looking like this
-lemma simulate'_tracking_oracle_query_equiv [spec.finite_range]
-  (s : S) : simulate' (⟪query | update_state, default_state⟫) oa s ≃ₚ oa :=
-begin
-  induction oa with A a A B oa ob hoa hob i t generalizing s,
-  { simp only [pure'_eq_pure, simulate'_pure, pure_map_equiv, eval_distribution_return] },
-  { let so := ⟪query | update_state, default_state⟫,
-    calc simulate' so (oa >>= ob) s
-      ≃ₚ simulate so oa s >>= λ x, simulate' so (ob x.1) x.2 : simulate'_bind_equiv _ oa ob _
-      ... ≃ₚ simulate so oa s >>= λ x, (ob x.1) : bind_equiv_of_equiv_second _ (by simp [hob])
-      ... ≃ₚ simulate' so oa s >>= ob : symm (bind_map_equiv _ prod.fst ob)
-      ... ≃ₚ oa >>= ob : bind_equiv_of_equiv_first ob (hoa _) },
-  { erw [simulate'_query_equiv, tracking_oracle_apply,
-      fst_map_bind_mk_equiv, map_id_equiv (query i t)], } 
-end
-
-end tracking_oracle
 
 section stateless_oracle
 
