src/computational_monads/simulation_semantics/constructions/tracking_oracle.lean
@@ -1,0 +1,50 @@
+import computational_monads.constructions.uniform_select
+import computational_monads.simulation_semantics.simulate
+
+open oracle_comp oracle_spec
+
+variables {A B : Type} {spec spec' spec'' : oracle_spec}
+  (oa : oracle_comp spec A)
+
+-- TODO: use namespaces to simplify the lemma names
+
+section tracking_oracle
+
+-- TODO: should be able to use `simps` everywhere instead of implementing projections
+
+/-- Oracle where the query result is indepenent of the current oracle state,
+  although the new state may depend upon the previous state.
+  For example a logging oracle that just tracks the input and output of queries. -/
+@[simps]
+def tracking_oracle {S : Type} (default_state : S)
+  (o : Π (i : spec.ι), spec.domain i → oracle_comp spec' (spec.range i))
+  (update_state : Π (s : S) (i : spec.ι), spec.domain i → spec.range i → S) :
+  simulation_oracle spec spec' :=
+{ S := S,
+  default_state := default_state,
+  o := λ i ⟨t, s⟩, do { u ← o i t, pure (u, update_state s i t u) } }
+
+notation `⟪` o `|` update_state `,` default_state `⟫` :=
+  tracking_oracle default_state o update_state
+
+variables {S : Type} (default_state : S)
+  (o : Π (i : spec.ι), spec.domain i → oracle_comp spec' (spec.range i))
+  (update_state : Π (s : S) (i : spec.ι), spec.domain i → spec.range i → S)
+
+-- TODO: should be able to find some generalization for lemmas looking like this
+lemma simulate'_tracking_oracle_query_equiv [spec.finite_range]
+  (s : S) : simulate' (⟪query | update_state, default_state⟫) oa s ≃ₚ oa :=
+begin
+  induction oa with A a A B oa ob hoa hob i t generalizing s,
+  { simp only [pure'_eq_pure, simulate'_pure, pure_map_equiv, eval_distribution_return] },
+  { let so := ⟪query | update_state, default_state⟫,
+    calc simulate' so (oa >>= ob) s
+      ≃ₚ simulate so oa s >>= λ x, simulate' so (ob x.1) x.2 : simulate'_bind_equiv _ oa ob _
+      ... ≃ₚ simulate so oa s >>= λ x, (ob x.1) : bind_equiv_of_equiv_second _ (by simp [hob])
+      ... ≃ₚ simulate' so oa s >>= ob : symm (bind_map_equiv _ prod.fst ob)
+      ... ≃ₚ oa >>= ob : bind_equiv_of_equiv_first ob (hoa _) },
+  { erw [simulate'_query_equiv, tracking_oracle_o,
+      fst_map_bind_mk_equiv, map_id_equiv (query i t)], } 
+end
+
+end tracking_oracle
